Added the rest of the examples

checks/Examples.v
@@ -1,8 +1,8 @@
-(* 
+(*
  * Examples.v
  * Wolf Honore
- * 
- * A set of example Tiger programs to be used in testing 
+ *
+ * A set of example Tiger programs to be used in testing
  * various parts of the compiler. Examples taken from those
  * provided by Zhong Shao in CPSC (4/5)21 (Yale).
  *)
@@ -406,3 +406,768 @@ Module EX19 <: EX.
                                StringExp " "]]]
       (SeqExp E[AppExp s_do_nothing1 E[IntExp 0; StringExp "str2"]]).
 End EX19.
+
+Module EX20 <: EX.
+(*
+/* error: undeclared variable i */
+
+while 10 > 5 do (i+1;())
+*)
+Definition s_i := sy 20.
+
+Definition ex : exp :=
+WhileExp (OpExp (IntExp 10) GtOp (IntExp 5))
+(SeqExp E[OpExp (VarExp (SimpleVar s_i)) PlusOp (IntExp 1);
+SeqExp E[]]).
+End EX20.
+
+Module EX21 <: EX.
+(*
+/* error : procedure returns value  and procedure is used in arexpr */
+let
+
+/* calculate n! */
+function nfactor(n: int) =
+		if  n = 0
+			then 1
+			else n * nfactor(n-1)
+
+in
+	nfactor(10)
+end
+
+*)
+Definition s_n := sy 20.
+Definition s_nfactor := sy 21.
+
+Definition ex : exp :=
+LetExp
+D[FunctionDec [Build_fundec s_nfactor [Build_formals (Build_vardec s_n true) Env.s_int]
+(None)]
+E[IfExp (OpExp (VarExp (SimpleVar s_n)) EqOp (IntExp 0))
+(IntExp 1)
+(Some (OpExp (VarExp (SimpleVar s_n)) TimesOp (AppExp s_nfactor E[OpExp (VarExp (SimpleVar s_n)) MinusOp (IntExp 1)])))]]
+(SeqExp E[AppExp s_nfactor E[IntExp 10]]).
+End EX21.
+
+Module EX22 <: EX.
+(*
+/* error : field not in record type */
+
+let
+	type rectype = {name:string , id:int}
+	var rec1 := rectype {name="Name", id=0}
+in
+	rec1.nam := "asd"
+end
+*)
+Definition s_nam := sy 20.
+Definition s_rec1 := sy 21.
+Definition s_id := sy 22.
+Definition s_name := sy 23.
+Definition s_rectype := sy 24.
+
+Definition ex : exp :=
+LetExp
+D[TypeDec [Build_tydec s_rectype (RecordTy [Build_tfield s_name Env.s_string;
+Build_tfield s_id Env.s_int])];
+VarDec (Build_vardec s_rec1 true) (None) (RecordExp E[StringExp "Name";
+IntExp 0]
+[s_name;
+s_id]
+s_rectype)]
+(SeqExp E[AssignExp (FieldVar (SimpleVar s_rec1) s_nam) (StringExp "asd")]).
+End EX22.
+
+Module EX23 <: EX.
+(*
+/* error : type mismatch */
+
+let
+	type rectype = {name:string , id:int}
+	var rec1 := rectype {name="aname", id=0}
+in
+	rec1.name := 3
+	rec1.id := ""
+end
+*)
+Definition s_rec1 := sy 20.
+Definition s_id := sy 21.
+Definition s_name := sy 22.
+Definition s_rectype := sy 23.
+
+Definition ex : exp :=
+LetExp
+D[TypeDec [Build_tydec s_rectype (RecordTy [Build_tfield s_name Env.s_string;
+Build_tfield s_id Env.s_int])];
+VarDec (Build_vardec s_rec1 true) (None) (RecordExp E[StringExp "aname";
+IntExp 0]
+[s_name;
+s_id]
+s_rectype)]
+(SeqExp E[AssignExp (FieldVar (SimpleVar s_rec1) s_name) (IntExp 3);
+AssignExp (FieldVar (SimpleVar s_rec1) s_id) (StringExp "")]).
+End EX23.
+
+Module EX24 <: EX.
+(*
+/* error : variable not array */
+let
+	var d:=0
+in
+	d[3]
+end
+
+*)
+Definition s_d := sy 20.
+
+Definition ex : exp :=
+LetExp
+D[VarDec (Build_vardec s_d true) (None) (IntExp 0)]
+(SeqExp E[VarExp (SubscriptVar (SimpleVar s_d) (IntExp 3))]).
+End EX24.
+
+Module EX25 <: EX.
+(*
+/* error : variable not record */
+let
+	var d:=0
+in
+	d.f
+end
+
+*)
+Definition s_f := sy 20.
+Definition s_d := sy 21.
+
+Definition ex : exp :=
+LetExp
+D[VarDec (Build_vardec s_d true) (None) (IntExp 0)]
+(SeqExp E[VarExp (FieldVar (SimpleVar s_d) s_f)]).
+End EX25.
+
+Module EX26 <: EX.
+(*
+/* error : integer required */
+
+3 + "var"
+*)
+Definition ex : exp :=
+OpExp (IntExp 3) PlusOp (StringExp "var").
+End EX26.
+
+Module EX27 <: EX.
+(*
+/* locals hide globals */
+let
+	var a:=0
+
+	function g(a:int):int = a
+in
+ g(2)
+end
+*)
+Definition s_g := sy 20.
+Definition s_a := sy 21.
+
+Definition ex : exp :=
+LetExp
+D[VarDec (Build_vardec s_a true) (None) (IntExp 0);
+FunctionDec [Build_fundec s_g [Build_formals (Build_vardec s_a true) Env.s_int]
+(Some Env.s_int)]
+E[VarExp (SimpleVar s_a)]]
+(SeqExp E[AppExp s_g E[IntExp 2]]).
+End EX27.
+
+Module EX28 <: EX.
+(*
+/* error : different record types */
+
+let
+	type rectype1 = {name:string , id:int}
+	type rectype2 = {name:string , id:int}
+
+	var rec1: rectype1 := rectype2 {name="Name", id=0}
+in
+	rec1
+end
+*)
+Definition s_rec1 := sy 20.
+Definition s_rectype2 := sy 21.
+Definition s_id := sy 22.
+Definition s_name := sy 23.
+Definition s_rectype1 := sy 24.
+
+Definition ex : exp :=
+LetExp
+D[TypeDec [Build_tydec s_rectype1 (RecordTy [Build_tfield s_name Env.s_string;
+Build_tfield s_id Env.s_int]);
+Build_tydec s_rectype2 (RecordTy [Build_tfield s_name Env.s_string;
+Build_tfield s_id Env.s_int])];
+VarDec (Build_vardec s_rec1 true) (Some s_rectype1) (RecordExp E[StringExp "Name";
+IntExp 0]
+[s_name;
+s_id]
+s_rectype2)]
+(SeqExp E[VarExp (SimpleVar s_rec1)]).
+End EX28.
+
+Module EX29 <: EX.
+(*
+/* error : different array types */
+
+let
+	type arrtype1 = array of int
+	type arrtype2 = array of int
+
+	var arr1: arrtype1 := arrtype2 [10] of 0
+in
+	arr1
+end
+*)
+Definition s_arr1 := sy 20.
+Definition s_arrtype2 := sy 21.
+Definition s_arrtype1 := sy 22.
+
+Definition ex : exp :=
+LetExp
+D[TypeDec [Build_tydec s_arrtype1 (ArrayTy Env.s_int);
+Build_tydec s_arrtype2 (ArrayTy Env.s_int)];
+VarDec (Build_vardec s_arr1 true) (Some s_arrtype1) (ArrayExp s_arrtype2
+(IntExp 10)
+(IntExp 0))]
+(SeqExp E[VarExp (SimpleVar s_arr1)]).
+End EX29.
+
+Module EX30 <: EX.
+(*
+/* synonyms are fine */
+
+let
+		type a = array of int
+		type b = a
+
+		var arr1:a := b [10] of 0
+in
+		arr1[2]
+end
+*)
+Definition s_arr1 := sy 20.
+Definition s_b := sy 21.
+Definition s_a := sy 22.
+
+Definition ex : exp :=
+LetExp
+D[TypeDec [Build_tydec s_a (ArrayTy Env.s_int);
+Build_tydec s_b (NameTy s_a)];
+VarDec (Build_vardec s_arr1 true) (Some s_a) (ArrayExp s_b
+(IntExp 10)
+(IntExp 0))]
+(SeqExp E[VarExp (SubscriptVar (SimpleVar s_arr1) (IntExp 2))]).
+End EX30.
+
+Module EX31 <: EX.
+(*
+/* error : type constraint and init value differ */
+let
+	var a:int := " "
+in
+	a
+end
+*)
+Definition s_a := sy 20.
+
+Definition ex : exp :=
+LetExp
+D[VarDec (Build_vardec s_a true) (Some Env.s_int) (StringExp " ")]
+(SeqExp E[VarExp (SimpleVar s_a)]).
+End EX31.
+
+Module EX32 <: EX.
+(*
+/* error : initializing exp and array type differ */
+
+let
+	type arrayty = array of int
+
+	var a := arrayty [10] of " "
+in
+	0
+end
+*)
+Definition s_a := sy 20.
+Definition s_arrayty := sy 21.
+
+Definition ex : exp :=
+LetExp
+D[TypeDec [Build_tydec s_arrayty (ArrayTy Env.s_int)];
+VarDec (Build_vardec s_a true) (None) (ArrayExp s_arrayty
+(IntExp 10)
+(StringExp " "))]
+(SeqExp E[IntExp 0]).
+End EX32.
+
+Module EX33 <: EX.
+(*
+/* error : unknown type */
+let
+	var a:= rectype {}
+in
+	0
+end
+*)
+Definition s_rectype := sy 20.
+Definition s_a := sy 21.
+
+Definition ex : exp :=
+LetExp
+D[VarDec (Build_vardec s_a true) (None) (RecordExp E[]
+[]
+s_rectype)]
+(SeqExp E[IntExp 0]).
+End EX33.
+
+Module EX34 <: EX.
+(*
+/* error : formals and actuals have different types */
+let
+	function g (a:int , b:string):int = a
+in
+	g("one", "two")
+end
+*)
+Definition s_b := sy 20.
+Definition s_a := sy 21.
+Definition s_g := sy 22.
+
+Definition ex : exp :=
+LetExp
+D[FunctionDec [Build_fundec s_g [Build_formals (Build_vardec s_a true) Env.s_int;
+Build_formals (Build_vardec s_b true) Env.s_string]
+(Some Env.s_int)]
+E[VarExp (SimpleVar s_a)]]
+(SeqExp E[AppExp s_g E[StringExp "one";
+StringExp "two"]]).
+End EX34.
+
+Module EX35 <: EX.
+(*
+/* error : formals are more then actuals */
+let
+	function g (a:int , b:string):int = a
+in
+	g("one")
+end
+*)
+Definition s_b := sy 20.
+Definition s_a := sy 21.
+Definition s_g := sy 22.
+
+Definition ex : exp :=
+LetExp
+D[FunctionDec [Build_fundec s_g [Build_formals (Build_vardec s_a true) Env.s_int;
+Build_formals (Build_vardec s_b true) Env.s_string]
+(Some Env.s_int)]
+E[VarExp (SimpleVar s_a)]]
+(SeqExp E[AppExp s_g E[StringExp "one"]]).
+End EX35.
+
+Module EX36 <: EX.
+(*
+/* error : formals are fewer then actuals */
+let
+	function g (a:int , b:string):int = a
+in
+	g(3,"one",5)
+end
+*)
+Definition s_b := sy 20.
+Definition s_a := sy 21.
+Definition s_g := sy 22.
+
+Definition ex : exp :=
+LetExp
+D[FunctionDec [Build_fundec s_g [Build_formals (Build_vardec s_a true) Env.s_int;
+Build_formals (Build_vardec s_b true) Env.s_string]
+(Some Env.s_int)]
+E[VarExp (SimpleVar s_a)]]
+(SeqExp E[AppExp s_g E[IntExp 3;
+StringExp "one";
+IntExp 5]]).
+End EX36.
+
+Module EX37 <: EX.
+(*
+/* redeclaration of variable, not an error */
+let
+	var a := 0
+	var a := " "
+in
+	0
+end
+*)
+Definition s_a := sy 20.
+
+Definition ex : exp :=
+LetExp
+D[VarDec (Build_vardec s_a true) (None) (IntExp 0);
+VarDec (Build_vardec s_a true) (None) (StringExp " ")]
+(SeqExp E[IntExp 0]).
+End EX37.
+
+Module EX38 <: EX.
+(*
+/* redeclaration of type error */
+let
+	type a = int
+	type a = string
+in
+	0
+end
+*)
+Definition s_a := sy 20.
+
+Definition ex : exp :=
+LetExp
+D[TypeDec [Build_tydec s_a (NameTy Env.s_int);
+Build_tydec s_a (NameTy Env.s_string)]]
+(SeqExp E[IntExp 0]).
+End EX38.
+
+Module EX39 <: EX.
+(*
+/* redeclaration of function error */
+let
+	function g(a:int):int = a
+	function g(a:int):int = a
+in
+	0
+end
+*)
+Definition s_a := sy 20.
+Definition s_g := sy 21.
+
+Definition ex : exp :=
+LetExp
+D[FunctionDec [Build_fundec s_g [Build_formals (Build_vardec s_a true) Env.s_int]
+(Some Env.s_int);
+Build_fundec s_g [Build_formals (Build_vardec s_a true) Env.s_int]
+(Some Env.s_int)]
+E[VarExp (SimpleVar s_a);
+VarExp (SimpleVar s_a)]]
+(SeqExp E[IntExp 0]).
+End EX39.
+
+Module EX40 <: EX.
+(*
+/* error : procedure returns value */
+let
+	function g(a:int) = a
+in
+	g(2)
+end
+
+*)
+Definition s_a := sy 20.
+Definition s_g := sy 21.
+
+Definition ex : exp :=
+LetExp
+D[FunctionDec [Build_fundec s_g [Build_formals (Build_vardec s_a true) Env.s_int]
+(None)]
+E[VarExp (SimpleVar s_a)]]
+(SeqExp E[AppExp s_g E[IntExp 2]]).
+End EX40.
+
+Module EX41 <: EX.
+(*
+/* local types hide global */
+let
+	type a = int
+in
+	let
+		type a = string
+	in
+		0
+	end
+end
+*)
+Definition s_a := sy 20.
+
+Definition ex : exp :=
+LetExp
+D[TypeDec [Build_tydec s_a (NameTy Env.s_int)]]
+(SeqExp E[LetExp
+D[TypeDec [Build_tydec s_a (NameTy Env.s_string)]]
+(SeqExp E[IntExp 0])]).
+End EX41.
+
+Module EX42 <: EX.
+(*
+/* correct declarations but with a syntax error */
+let
+
+type arrtype1 = array of int
+type rectype1 = {name:string, address:string, id: int , age: int}
+type arrtype2 = array of rectype1
+type rectype2 = {name : string, dates: arrtype1}
+
+type arrtype3 = array of string
+
+var arr1 := arrtype1 [10] of 0
+var arr2  := arrtype2 [5] of rectype1 {name="aname", address="somewhere", id=0, age=0}}
+var arr3:arrtype3 := arrtype3 [100] of ""
+
+var rec1 := rectype1 {name="Kapoios", address="Kapou", id=02432, age=44}
+var rec2 := rectype2 {name="Allos", dates= arrtype1 [3] of 1900}
+
+in
+
+arr1[0] := 1;
+arr1[9] := 3;
+arr2[3].name := "kati";
+arr2[1].age := 23;
+arr3[34] := "sfd";
+
+rec1.name := "sdf";
+rec2.dates[0] := 2323;
+rec2.dates[2] := 2323
+
+end
+*)
+Definition s_rec2 := sy 20.
+Definition s_rec1 := sy 21.
+Definition s_arr3 := sy 22.
+Definition s_arr2 := sy 23.
+Definition s_arr1 := sy 24.
+Definition s_arrtype3 := sy 25.
+Definition s_dates := sy 26.
+Definition s_rectype2 := sy 27.
+Definition s_arrtype2 := sy 28.
+Definition s_age := sy 29.
+Definition s_id := sy 30.
+Definition s_address := sy 31.
+Definition s_name := sy 32.
+Definition s_rectype1 := sy 33.
+Definition s_arrtype1 := sy 34.
+
+Definition ex : exp :=
+LetExp
+D[TypeDec [Build_tydec s_arrtype1 (ArrayTy Env.s_int);
+Build_tydec s_rectype1 (RecordTy [Build_tfield s_name Env.s_string;
+Build_tfield s_address Env.s_string;
+Build_tfield s_id Env.s_int;
+Build_tfield s_age Env.s_int]);
+Build_tydec s_arrtype2 (ArrayTy s_rectype1);
+Build_tydec s_rectype2 (RecordTy [Build_tfield s_name Env.s_string;
+Build_tfield s_dates s_arrtype1]);
+Build_tydec s_arrtype3 (ArrayTy Env.s_string)];
+VarDec (Build_vardec s_arr1 true) (None) (ArrayExp s_arrtype1
+(IntExp 10)
+(IntExp 0));
+VarDec (Build_vardec s_arr2 true) (None) (ArrayExp s_arrtype2
+(IntExp 5)
+(RecordExp E[StringExp "aname";
+StringExp "somewhere";
+IntExp 0;
+IntExp 0]
+[s_name;
+s_address;
+s_id;
+s_age]
+s_rectype1));
+VarDec (Build_vardec s_arr3 true) (Some s_arrtype3) (ArrayExp s_arrtype3
+(IntExp 100)
+(StringExp ""));
+VarDec (Build_vardec s_rec1 true) (None) (RecordExp E[StringExp "Kapoios";
+StringExp "Kapou";
+IntExp 2432;
+IntExp 44]
+[s_name;
+s_address;
+s_id;
+s_age]
+s_rectype1);
+VarDec (Build_vardec s_rec2 true) (None) (RecordExp E[StringExp "Allos";
+ArrayExp s_arrtype1
+(IntExp 3)
+(IntExp 1900)]
+[s_name;
+s_dates]
+s_rectype2)]
+(SeqExp E[AssignExp (SubscriptVar (SimpleVar s_arr1) (IntExp 0)) (IntExp 1);
+AssignExp (SubscriptVar (SimpleVar s_arr1) (IntExp 9)) (IntExp 3);
+AssignExp (FieldVar (SubscriptVar (SimpleVar s_arr2) (IntExp 3)) s_name) (StringExp "kati");
+AssignExp (FieldVar (SubscriptVar (SimpleVar s_arr2) (IntExp 1)) s_age) (IntExp 23);
+AssignExp (SubscriptVar (SimpleVar s_arr3) (IntExp 34)) (StringExp "sfd");
+AssignExp (FieldVar (SimpleVar s_rec1) s_name) (StringExp "sdf");
+AssignExp (SubscriptVar (FieldVar (SimpleVar s_rec2) s_dates) (IntExp 0)) (IntExp 2323);
+AssignExp (SubscriptVar (FieldVar (SimpleVar s_rec2) s_dates) (IntExp 2)) (IntExp 2323)]).
+End EX42.
+
+Module EX43 <: EX.
+(*
+/* initialize with unit and causing type mismatch in addition */
+
+let
+	var a := ()
+in
+	a + 3
+end
+*)
+Definition s_a := sy 20.
+
+Definition ex : exp :=
+LetExp
+D[VarDec (Build_vardec s_a true) (None) (SeqExp E[])]
+(SeqExp E[OpExp (VarExp (SimpleVar s_a)) PlusOp (IntExp 3)]).
+End EX43.
+
+Module EX44 <: EX.
+(*
+/* valid nil initialization and assignment */
+let
+
+	type rectype = {name:string, id:int}
+	var b:rectype := nil
+
+in
+
+	b := nil
+
+end
+*)
+Definition s_b := sy 20.
+Definition s_id := sy 21.
+Definition s_name := sy 22.
+Definition s_rectype := sy 23.
+
+Definition ex : exp :=
+LetExp
+D[TypeDec [Build_tydec s_rectype (RecordTy [Build_tfield s_name Env.s_string;
+Build_tfield s_id Env.s_int])];
+VarDec (Build_vardec s_b true) (Some s_rectype) (NilExp)]
+(SeqExp E[AssignExp (SimpleVar s_b) (NilExp)]).
+End EX44.
+
+Module EX45 <: EX.
+(*
+/* error: initializing nil expressions not constrained by record type + syntax error */
+let
+	type rectype = {name:string, id:int}
+
+	var a:= rectype nil
+	var a:= nil
+in
+	a
+end
+*)
+Definition s_a := sy 20.
+Definition s_id := sy 21.
+Definition s_name := sy 22.
+Definition s_rectype := sy 23.
+
+Definition ex : exp :=
+LetExp
+D[TypeDec [Build_tydec s_rectype (RecordTy [Build_tfield s_name Env.s_string;
+Build_tfield s_id Env.s_int])];
+VarDec (Build_vardec s_a true) (None) (OpExp (VarExp (SimpleVar s_rectype)) PlusOp (NilExp));
+VarDec (Build_vardec s_a true) (None) (NilExp)]
+(SeqExp E[VarExp (SimpleVar s_a)]).
+End EX45.
+
+Module EX46 <: EX.
+(*
+/* validity of rec comparisons */
+let
+	type rectype = {name:string, id:int}
+	var b:rectype := nil
+in
+	nil=nil;   /* this line should be rejected by your typechecker */
+	b= nil;
+	b <> nil
+end
+*)
+Definition s_b := sy 20.
+Definition s_id := sy 21.
+Definition s_name := sy 22.
+Definition s_rectype := sy 23.
+
+Definition ex : exp :=
+LetExp
+D[TypeDec [Build_tydec s_rectype (RecordTy [Build_tfield s_name Env.s_string;
+Build_tfield s_id Env.s_int])];
+VarDec (Build_vardec s_b true) (Some s_rectype) (NilExp)]
+(SeqExp E[OpExp (NilExp) EqOp (NilExp);
+OpExp (VarExp (SimpleVar s_b)) EqOp (NilExp);
+OpExp (VarExp (SimpleVar s_b)) NeqOp (NilExp)]).
+End EX46.
+
+Module EX47 <: EX.
+(*
+/* error : invalid recursion  */
+let
+	type a = int
+
+	var d:=0
+
+	type a = a
+in
+	0
+end
+*)
+Definition s_d := sy 20.
+Definition s_a := sy 21.
+
+Definition ex : exp :=
+LetExp
+D[TypeDec [Build_tydec s_a (NameTy Env.s_int)];
+VarDec (Build_vardec s_d true) (None) (IntExp 0);
+TypeDec [Build_tydec s_a (NameTy s_a)]]
+(SeqExp E[IntExp 0]).
+End EX47.
+
+Module EX48 <: EX.
+(*
+/* valid let with unit body */
+let
+in
+end
+*)
+Definition ex : exp :=
+LetExp
+D[]
+(SeqExp E[]).
+End EX48.
+
+Module EX49 <: EX.
+(*
+/* valid type decs */
+
+let
+	type i =int
+
+	var t:=0
+
+	type a = b
+	type b = c
+	type c = i
+
+in
+end
+*)
+Definition s_c := sy 20.
+Definition s_b := sy 21.
+Definition s_a := sy 22.
+Definition s_t := sy 23.
+Definition s_i := sy 24.
+
+Definition ex : exp :=
+LetExp
+D[TypeDec [Build_tydec s_i (NameTy Env.s_int)];
+VarDec (Build_vardec s_t true) (None) (IntExp 0);
+TypeDec [Build_tydec s_a (NameTy s_b);
+Build_tydec s_b (NameTy s_c);
+Build_tydec s_c (NameTy s_i)]]
+(SeqExp E[]).
+End EX49.
